

$$1) a) 1 - P(\text{no rain}) = 1 - 0.3$$

$$= 1 - 0.4 \cdot 0.5 = 0.7 = P(A \cup B)$$

$$b) P(A \cap B) = P(A) + P(B) - P(A \cup B)$$

$$= 0.6 + 0.5 - 0.7$$

$$= 0.4$$

$$c) P(A \cap \bar{B}) = P(A \cup B) - P(B)$$

$$= 0.7 - 0.5 = 0.2$$

$$d) P(A \cup B) - P(A \cap B) = 0.3$$

$$2) S = \{1, 2, 3, 4, 5, 6\} \times \{1, 2, 3, 4, 5, 6\}$$

$$P(A) = 5/36$$

$$3) h - \text{probability of girl (usually } 1/2)$$

$$P(\text{choosing a girl}) = \frac{1}{2} = \sum_{n=1}^{\infty} \frac{1}{n} \binom{n}{n-1} h^n (1-h)^{n-n}$$

$$= \sum_{n=1}^{\infty} \binom{n-1}{n-1} h^n (1-h)^{n-n}$$

$$= h \sum_{n=1}^{\infty} \binom{n-1}{n-1} h^{n-1} (1-h)^{n-n}$$

$$= h$$

$$p = \frac{1 \cdot {}^n C_n h^n}{h^{n-1}}$$

$$h = \frac{1}{2}$$

$$p = \frac{1}{2^{n-1}}$$

$$4) \quad X \begin{cases} X_d & \text{with } h \\ X_c & \text{with } 1-h \end{cases}$$

$$1) \quad F_X(x) = P(X < x) = h \cdot P(X_d < x) + (1-h) \cdot P(X_c < x) \\ = h F_d(x) + (1-h) F_c(x)$$

$$2) \quad f_X(x) = h f_d(x) + (1-h) f_c(x)$$

$$3) \quad E[X] = \int x f_X(x) dx \\ = h E[X_d] + (1-h) E[X_c]$$

$$4) \quad \text{Var } X = E[X^2] - E^2[X]$$

$$= \int x^2 f_X(x) dx = h E[X_d^2] + (1-h) E[X_c^2] + h(1-h)(E[X_d] - E[X_c])^2$$

$$5) \quad Z = 1 + X + XY^2, \quad W = 1 + X$$

$$\text{Cov}(Z, W) = E(ZW) - E(Z)E(W)$$

$$= E[(1+X+XY^2)(1+X)] - E[1+X+XY^2]E[1+X]$$

$$= E[1+X+XY^2+X+X^2+X^2Y^2] - 1 = 1 + 1 + 1 + 1 + 1 + 1 - 1 = 6 - 1 = 5$$

$$6) P(\geq 1 \text{ offer}) = 1 - P(\text{no offer}) \\ = 1 - (0.8)^4 \quad (\text{Assuming independence}) \\ = \cancel{0.4096} 0.59$$

$$P(A \cup B \cup C \cup D) \leq \sum P(X_i) \\ \leq 0.2 \times 4 = 0.8$$

$$\text{So } P(\geq 1 \text{ offer}) \leq 0.8 \\ \text{So he is wrong.}$$

$$7) \frac{S_n - n\mu}{\sqrt{n}\sigma} \rightarrow N(0,1) \text{ as } n \text{ is large.}$$

$$\mu = p = 0.1 \quad \sigma^2 = h(1-h) = 0.1 \times 0.9 \\ \sigma^2 = 0.09 \\ \sigma = 0.3$$

$$S_n \geq 120 \Rightarrow S_n \geq 121$$

$$N(0,1) \geq \frac{121 - 100}{\sqrt{1000} \cdot 0.3} = 2.21 \\ \approx 0.0136$$

13.6 % chance

$$8) \text{ CLT again } \mu = 1, \sigma = \frac{1}{\sqrt{2}}$$

$$\& \text{ For } 64 \Rightarrow \mu = 64, \sigma = \sqrt{32} = 5.66$$

$$z = 1.645 \text{ for } 95\%, 64 + 1.645 \times 5.66 \\ = 74 \text{ sandwich}$$

$$9) 1) 0, 0$$

$$2) 1, 1$$

$$3) 1, 1$$

$$10) E[X|Y=y] = \mu_x + \frac{\text{Cov}(X,Y)}{\text{Var } Y} (y - \mu_y)$$

$$= 1 + \frac{1}{3} (y - 2)$$

$$\text{Var}[X|Y=y] = \sigma_x^2 - \frac{\text{Cov}^2(X,Y)}{\sigma_y^2}$$

$$= 4 - \frac{1}{3} = \frac{11}{3}$$

$$X \left(1 + \frac{1}{3} (y - 2), \frac{11}{3} \right)$$

11) X, Y are jointly Gaussian, their linear combⁿ is Gaussian too.

$$E[Z] = 0 \quad \text{Var}[Z] = 9 \text{Var}[X] + 4 \text{Var}[Y] - 2 \text{Cov}(X, 2Y)$$

$$\text{Var}[Z] = 9 \text{Var}[X] + 4 \text{Var}[Y] - 2 \text{Cov}(X, 2Y)$$

$$= 9 + 16 - 2 \times 3 \times 2 = 13$$

$$Z \sim N(0, 13)$$

$$\rho = \frac{E[ZX] - E[Z]E[X]}{\sqrt{\sigma_z^2 \sigma_x^2}} = \frac{E[3x^2 - 2xy]}{\sqrt{13}}$$

$$= \frac{3 \times 1 - 2}{\sqrt{13}} = \frac{1}{\sqrt{13}}$$

$$12) \mu_x = \mu_x +$$

$$\Sigma = \begin{bmatrix} \Sigma_{11} & \Sigma_{12} \\ \Sigma_{21} & \Sigma_{22} \end{bmatrix}$$

$$\Sigma \begin{pmatrix} x \\ y \\ z \end{pmatrix} = \begin{matrix} \Sigma_{11} & \Sigma_{12} \\ \Sigma_{21} & \Sigma_{22} \end{matrix}$$

$$\bar{\mu} = \mu_1 + \Sigma_{12} \Sigma_{22}^{-1} (a - \mu_2)$$

$$a = \begin{pmatrix} y \\ z \end{pmatrix} \quad \Sigma_{22}^{-1} = \frac{1}{14} \begin{pmatrix} 5 & 1 \\ 1 & 3 \end{pmatrix}$$

$$\begin{pmatrix} 2 & 1 \end{pmatrix} \frac{1}{14} \begin{pmatrix} 5 & 1 \\ 1 & 3 \end{pmatrix} = \frac{1}{14} \begin{pmatrix} 11 & 5 \end{pmatrix}$$

$$\frac{1}{14} [11(y - 0) + 5(z - 0)]$$

$$= \frac{1}{14} [11y + 5z]$$

$$\bar{\mu} = \frac{0 + 11y + 5z}{14} = \frac{11y + 5z}{14}$$

$$\bar{\Sigma} = \Sigma_{11} - \Sigma_{12} \Sigma_{22}^{-1} \Sigma_{21}$$

$$= 4 - \frac{1}{14} (11 \quad 5) \begin{pmatrix} 2 \\ 1 \end{pmatrix}$$

$$\text{Var}(X) = 4 - \frac{27}{14}$$

$$= \frac{29}{14}$$

$$\cancel{X} \sim \left(\frac{11y + 53}{14}, \frac{29}{14} \right) \in \mathbb{R} \text{ is one}$$

$$4) 4) E[X^2] - E^2[X]$$

$$= h E[X_d^2] + (1-h) E[X_c^2]$$

$$= h^2 E^2[X_d] + (1-h)^2 E^2[X_c]$$

$$- 2h(1-h) E[X_d] E[X_c]$$

$$= h \text{Var}(X_d) + (1-h) \text{Var}(X_c) + h E^2[X_d] + (1-h) E^2[X_c] - h E^2[X_d]$$

$$E^2[X_d] h(-h) + h(1-h) E^2[X_c] - 2h(1-h) E[X_d] E[X_c]$$

$$= h(1-h) (E[X_d] - E[X_c])^2 + h \text{Var}(X_d) + (1-h) \text{Var}(X_c)$$